Invoke & closedness

Syntax.v
@@ -2,6 +2,7 @@ Require Import List.
 Import ListNotations.
 Require Import Arith.
 Require Import Omega.
+Require Eqdep_dec Arith.
 Require Import Unify.
 
 Inductive goal : Set :=
@@ -10,6 +11,29 @@ Inductive goal : Set :=
 (* conjunction *) | Conj   : goal -> goal -> goal
 (* fresh       *) | Fresh  : (name -> goal) -> goal
 (* invoke      *) | Invoke : name -> list term -> goal.
+
+(* Free variable monadic enumerator *)
+Fixpoint fvm (n : name) (g : goal) : list name * name :=
+  match g with
+  | Unify t1 t2 => (fv_term t1 ++ fv_term t2, n)
+  | Disj  g1 g2
+  | Conj  g1 g2 => let (t1, n1) := fvm n  g1 in
+                   let (t2, n2) := fvm n1 g2 in
+                   (t1 ++ t2, n2)
+  | Fresh fg    => let g := fg n in
+                   let (ts, n') := fvm (S n) g in
+                   (remove Nat.eq_dec n ts, n')
+  | Invoke _ ts => (fv_terms ts, n)
+  end.
+
+(* Free variables enumerator *)
+Definition fv_goal n g := fst (fvm n g).
+
+(* Closedness of goals *)
+Definition closed_goal_in_context (c : list name) (g : goal) : Prop :=
+  forall x, (forall n, In x (fv_goal n g)) -> In x c.
+
+Definition closed_goal : goal -> Prop := closed_goal_in_context [].
 
 (* N-ary function type from term to goals *)
 Fixpoint n_ary (n : nat) : Set :=
@@ -26,21 +50,96 @@ revert args. induction n.
   + inversion H.
   + inversion H. refine (IHn (f t) args H1).
 Defined.
-
+           
 (* rel is a body of a relational symbol *)
 Inductive rel : Set :=
-  Def : forall n, n_ary n -> rel.
+  Rel : forall n, n_ary n -> rel.
+
+(* Arity of a relational symbol *)
+Definition arity (r : rel) : nat :=
+  match r with
+  | Rel n _ => n
+  end.
+
+(* Application of a relational symbol *)
+Definition apply_rel (r : rel) (args : list term) (c : length args = arity r) : goal.
+  destruct r eqn:R. simpl in c. apply (n_apply n n0 args c).
+Defined.
+
+(* Closedness of a relational symbol *)
+Definition closed_rel (r : rel) : Prop :=
+  forall (args : list term) (c : length args = arity r),
+    closed_goal_in_context (fv_terms args) (apply_rel r args c).
 
 (* Some checks *)
-Definition d0 : rel := Def 0 (           Unify (Var 0) (Var 0)).
-Definition d1 : rel := Def 1 (fun t   => Unify t       (Var 0)).
-Definition d2 : rel := Def 2 (fun t q => Unify t       q      ).
+Module SmokeTest.
 
-(* def is a definition of a relational symbol *)
-Definition def : Set := name * rel.
+  Definition g0 : goal := Fresh (fun x => Unify (Var x) (Cst 2)).
+  Definition g1 : goal := Fresh (fun x => Fresh (fun y => Unify (Var x) (Var y))).
+
+  Lemma g0_closed : closed_goal g0.
+  Proof.
+    unfold closed_goal. unfold closed_goal_in_context. intros x H.
+    unfold fv_goal in H. unfold fvm in H. unfold g0 in H. simpl in H.
+    specialize (H x). destruct (Nat.eq_dec x x) eqn:D. assumption. contradiction.
+  Qed.
+  
+  Lemma g1_closed : closed_goal g1.
+  Proof.
+    unfold closed_goal. unfold closed_goal_in_context. intros x H.
+    unfold fv_goal in H. unfold fvm in H. unfold g1 in H. unfold fv_term in H.
+    specialize (H x). simpl in H. destruct (Nat.eq_dec x x) eqn:D. destruct x. simpl in H. auto.
+    destruct (Nat.eq_dec (S x) x). simpl in H. auto. simpl in H. destruct (Nat.eq_dec x x). auto. contradiction. contradiction.
+  Qed.
+    
+  Definition r0 : rel := Rel 0 (           Unify (Cst 0) (Cst 0)).
+  Definition r1 : rel := Rel 1 (fun t   => Fresh (fun q => Unify t (Var q))).
+  Definition r2 : rel := Rel 2 (fun t q => Unify t q).
+
+  Lemma r0_closed : closed_rel r0.
+  Proof.
+    unfold closed_rel. intros. simpl in c. destruct args eqn:A.
+    * unfold fv_terms. simpl. unfold closed_goal_in_context. simpl. auto.
+    * simpl in c. inversion c.
+  Qed.
+
+  Lemma r1_closed : closed_rel r1.
+  Proof.
+    unfold closed_rel. intros. simpl in c. destruct args eqn:A.
+    * simpl in c. inversion c.
+    * simpl in c. inversion c. unfold length in H0. destruct l eqn:L.
+      + simpl in c.
+        assert (App: apply_rel r1 [t] c = Fresh (fun q => Unify t (Var q))).
+          simpl. replace c with (eq_refl 1). auto. apply Eqdep_dec.UIP_dec, eq_nat_dec.  (* Wow! Wow! *)
+        rewrite App. unfold fv_terms. simpl. unfold closed_goal_in_context. intros. unfold fv_goal in H.
+        unfold fvm in H. simpl in H. remember (free_var t) as FV. inversion_clear FV.
+        specialize (H x0).
+        assert (HH: remove Nat.eq_dec x0 (fv_term t ++ [x0]) = fv_term t). admit.
+        rewrite <-HH. auto.
+      + simpl in c. inversion c.
+  Admitted.
+    
+  Lemma r2_closed : closed_rel r2.
+  Proof.
+    unfold closed_rel. intros. simpl in c. unfold length in c. destruct args eqn:A.
+    * inversion c.
+    * destruct l. inversion c.
+      + destruct l.
+         - assert (App: apply_rel r2 [t; t0] c = Unify t t0).
+             simpl. replace c with (eq_refl 2). simpl. reflexivity. apply Eqdep_dec.UIP_dec, eq_nat_dec. (* Wow! Wow! *)
+           rewrite App. unfold fv_terms. simpl. unfold closed_goal_in_context. intros. unfold fv_goal in H.
+           unfold fvm in H. simpl in H. auto.
+         - inversion c.
+  Qed.
+  
+End SmokeTest.
+
+(* def is a definition of a closed relational symbol *)
+Inductive def : Set :=
+  Def : forall (r: rel), closed_rel r -> def.
 
 (* spec is a list of definitions *)
-Definition spec : Set := list def.
+Definition spec : Set := list (name * def).
 
 (* Partial state *) 
 Inductive state' : Set :=
@@ -64,18 +163,21 @@ Section Transitions.
   Variable P : spec.
 
   Inductive eval_step : state' -> label -> state -> Prop :=
-  | UnifyFail    : forall t1 t2 s    n, MGU (apply s t1) (apply s t2) None      -> eval_step (Leaf (Unify t1 t2) s n) Step Stop
-  | UnifySuccess : forall t1 t2 s s' n, MGU (apply s t1) (apply s t2) (Some s') -> eval_step (Leaf (Unify t1 t2) s n) (Answer (compose s' s) n) Stop
-  | DisjS        : forall g1 g2       s n, eval_step (Leaf (Disj g1 g2) s n) Step (State (Sum (Leaf g1 s n) (Leaf g2 s n)))
-  | ConjS        : forall g1 g2       s n, eval_step (Leaf (Conj g1 g2) s n) Step (State (Prod (Leaf g1 s n) g2))
-  | FreshS       : forall fg          s n, eval_step (Leaf (Fresh fg) s n) Step (State (Leaf (fg n) s (S n)))
-  | InvokeS      : forall f args (rf : n_ary (length args)) s n, find (fun x => Nat.eqb (fst x) f) P = Some (f, Def (length args) rf) ->
-                                                                 eval_step (Leaf (Invoke f args) s n) Step (State (Leaf (n_apply (length args) rf args (eq_refl (length args))) s n))
-  | SumE         : forall st1 st2      l, eval_step st1 l  Stop        -> eval_step (Sum st1 st2) l (State st2)
-  | SumNE        : forall st1 st1' st2 l, eval_step st1 l (State st1') -> eval_step (Sum st1 st2) l (State (Sum st2 st1'))
-  | ProdSE       : forall st g,         eval_step st  Step         Stop       -> eval_step (Prod st g) Step Stop
-  | ProdAE       : forall st g s n,     eval_step st (Answer s n)  Stop       -> eval_step (Prod st g) Step (State (Leaf g s n))
-  | ProdSNE      : forall st g     st', eval_step st  Step        (State st') -> eval_step (Prod st g) Step (State (Prod st' g))
-  | ProdANE      : forall st g s n st', eval_step st (Answer s n) (State st') -> eval_step (Prod st g) Step (State (Sum (Leaf g s n) (Prod st' g))).
+  | UnifyFail    : forall t1 t2     s    n , MGU (apply s t1) (apply s t2) None      -> eval_step (Leaf (Unify t1 t2) s n) Step Stop
+  | UnifySuccess : forall t1 t2     s s' n , MGU (apply s t1) (apply s t2) (Some s') -> eval_step (Leaf (Unify t1 t2) s n) (Answer (compose s' s) n) Stop
+  | DisjS        : forall g1 g2        s n , eval_step (Leaf (Disj g1 g2) s n) Step (State (Sum (Leaf g1 s n) (Leaf g2 s n)))
+  | ConjS        : forall g1 g2        s n , eval_step (Leaf (Conj g1 g2) s n) Step (State (Prod (Leaf g1 s n) g2))
+  | FreshS       : forall fg           s n , eval_step (Leaf (Fresh fg) s n)   Step (State (Leaf (fg n) s (S n)))
+                                                       
+  | InvokeS      : forall f args r s n (c : length args = arity r) (cl : closed_rel r),
+                     find (fun x => Nat.eqb (fst x) f) P = Some (f, Def r cl) -> 
+                     eval_step (Leaf (Invoke f args) s n) Step (State (Leaf (apply_rel r args c) s n))
+                                                      
+  | SumE         : forall st1 st2        l , eval_step st1 l  Stop                    -> eval_step (Sum st1 st2) l (State st2)
+  | SumNE        : forall st1 st1' st2   l , eval_step st1 l (State st1')             -> eval_step (Sum st1 st2) l (State (Sum st2 st1'))
+  | ProdSE       : forall st g             , eval_step st     Step         Stop       -> eval_step (Prod st g) Step Stop
+  | ProdAE       : forall st g s n         , eval_step st    (Answer s n)  Stop       -> eval_step (Prod st g) Step (State (Leaf g s n))
+  | ProdSNE      : forall st g     st'     , eval_step st     Step        (State st') -> eval_step (Prod st g) Step (State (Prod st' g))
+  | ProdANE      : forall st g s n st'     , eval_step st    (Answer s n) (State st') -> eval_step (Prod st g) Step (State (Sum (Leaf g s n) (Prod st' g))).
 
 End Transitions.
